src/ndep/SymEval.v
@@ -7,6 +7,244 @@ Set Strict Implicit.
 
 Definition W := word 32.
 
+Section UpdatePosition.
+  Variable T : Type.
+
+  Fixpoint updatePosition (n : nat) (v : T) (ls : list T) : list T :=
+    match n , ls with
+      | 0 , nil => v :: nil
+      | 0 , _ :: b => v :: b 
+      | S n , nil => v :: updatePosition n v nil
+      | S n , a :: b => a :: updatePosition n v b
+    end.
+
+  Lemma updatePosition_eq : forall n types' t,
+    nth_error (updatePosition n t types') n = Some t.
+  Proof.
+    induction n; simpl; destruct types'; eauto.
+  Defined.
+
+  Lemma updatePosition_neq : forall t n types' m,
+    n <> m ->
+    nth_error types' n <> None ->
+    nth_error (updatePosition m t types') n = nth_error types' n.
+  Proof.
+    clear.
+    induction n; destruct types'; destruct m; simpl; intros; try solve [ exfalso; auto; omega ]; auto.
+  Defined.
+End UpdatePosition.
+
+(** * These are generic search functions *)
+Section search_read_write.
+  Variable A : Type.
+  Variable B : A -> Type.
+  Variable types : list type.
+  Variable sfuncs : list A.
+
+
+  Variable T : Type.
+  Variable F : forall s, B s -> list (expr types) -> option T.
+  Variable F_upd : forall s, B s -> list (expr types) -> option (list (expr types)).
+
+  Section arg.
+    Variable ss : A.
+    Variable se : B ss.
+    
+    Fixpoint fold_args (es : list (list (expr types))) : option T :=
+      match es with 
+        | nil => None
+        | a :: b => 
+          match F se a with
+            | None => fold_args b
+            | Some r => Some r
+          end
+      end.
+    
+    Theorem fold_args_correct : forall es v,
+      fold_args es = Some v ->
+      exists k, In k es /\ F se k = Some v.
+    Proof.
+      clear. induction es.
+      simpl; congruence.
+      simpl. case_eq (F se a); intros.
+      inversion H0. subst. eauto.
+      eapply IHes in H0. destruct H0.
+      exists x. tauto.
+    Qed.
+
+    Fixpoint fold_args_update (es : list (list (expr types))) : option (list (list (expr types))) :=
+      match es with 
+        | nil => None
+        | a :: b => 
+          match F_upd se a with
+            | None => match fold_args_update b with
+                        | None => None
+                        | Some b => Some (a :: b)
+                      end
+            | Some r => Some (r :: b)
+          end
+      end.
+    
+    Theorem fold_args_update_correct : forall es es',
+      fold_args_update es = Some es' ->
+      exists pre, exists post, exists k, exists k',
+        es = pre ++ k :: post /\
+        F_upd se k = Some k' /\
+        es' = pre ++ k' :: post.
+    Proof.
+      clear. induction es.
+      simpl; congruence.
+      simpl. case_eq (F_upd se a); intros.
+      inversion H0. subst. do 4 eexists; intuition eauto.
+      instantiate (2 := nil). reflexivity. reflexivity.
+
+      generalize dependent H0.
+      case_eq (fold_args_update es); intros.
+      inversion H1; subst. eapply IHes in H0.
+      do 4 destruct H0. exists (a :: x). exists x0.
+      eexists; eexists; intuition; subst; eauto. reflexivity.
+
+      congruence.
+    Qed.
+
+    
+
+  End arg.
+
+  Variable impures : FM.t (list (list (expr types))).
+
+  Fixpoint fold_known (k : list nat) :
+    hlist (fun n : nat => match nth_error sfuncs n with
+                            | None => Empty_set 
+                            | Some ss => B ss
+                          end) k
+    -> option T :=
+    match k as k 
+      return hlist (fun n : nat => match nth_error sfuncs n with
+                                     | None => Empty_set 
+                                     | Some ss => B ss
+                                   end) k
+      -> option T
+      with
+      | nil => fun _ => None
+      | a :: b => fun ss =>
+        match FM.find a impures with
+          | None => fold_known (hlist_tl ss)
+          | Some argss =>
+            match nth_error sfuncs a as ss
+              return match ss with
+                       | None => Empty_set 
+                       | Some ss => B ss
+                     end -> option T
+              with
+              | Some _ => fun se =>
+                match fold_args se argss with
+                  | None => fold_known (hlist_tl ss)
+                  | Some r => Some r
+                end
+              | None => fun err => match err with end
+            end (hlist_hd ss)
+        end
+    end.
+  
+  Theorem fold_known_correct : forall k
+    (h : hlist (fun n : nat => match nth_error sfuncs n with
+                                 | None => Empty_set 
+                                 | Some ss => B ss
+                               end) k) v,
+    @fold_known k h = Some v ->
+    exists n, exists ss,
+      exists se :  B ss, exists ls, exists args, 
+        nth_error sfuncs n = Some ss 
+        /\ FM.find n impures = Some ls 
+        /\ In args ls 
+        /\ F se args = Some v.
+  Proof.
+    clear. induction k; simpl.
+    congruence.
+    intros h v. specialize (IHk (hlist_tl h) v).
+    rewrite (hlist_eta _ h) in *.
+    generalize dependent (hlist_hd h). simpl.
+    case_eq (FM.find a impures); intros; eauto 10.
+
+    assert (exists k, nth_error sfuncs a = Some k).
+    generalize y. clear.
+    destruct (nth_error sfuncs a); [ eauto | destruct 1 ]. 
+    destruct H1.
+    generalize dependent y.
+    rewrite H1. intro.
+    case_eq (fold_args y l); intros; eauto 10.
+    inversion H2; subst.
+    eapply fold_args_correct in H0. destruct H0; eauto 10.
+  Qed.
+
+  Fixpoint fold_known_update (k : list nat) :
+    hlist (fun n : nat => match nth_error sfuncs n with
+                            | None => Empty_set 
+                            | Some ss => B ss
+                          end) k
+    -> option (FM.t (list (list (expr types)))) :=
+    match k as k 
+      return hlist (fun n : nat => match nth_error sfuncs n with
+                                     | None => Empty_set 
+                                     | Some ss => B ss
+                                   end) k
+      -> option (FM.t (list (list (expr types))))
+      with
+      | nil => fun _ => None
+      | a :: b => fun ss =>
+        match FM.find a impures with
+          | None => fold_known_update (hlist_tl ss)
+          | Some argss =>
+            match nth_error sfuncs a as ss
+              return match ss with
+                       | None => Empty_set 
+                       | Some ss => B ss
+                     end -> option (FM.t (list (list (expr types))))
+              with
+              | Some _ => fun se =>
+                match fold_args_update se argss with
+                  | None => fold_known_update (hlist_tl ss)
+                  | Some r => Some (FM.add a r impures) (* this is a replace *)
+                end
+              | None => fun err => match err with end
+            end (hlist_hd ss)
+        end
+    end.
+  
+  Theorem fold_known_update_correct : forall k
+    (h : hlist (fun n : nat => match nth_error sfuncs n with
+                                 | None => Empty_set 
+                                 | Some ss => B ss
+                               end) k) i',
+    @fold_known_update k h = Some i' ->
+    exists n, exists ss,
+      exists se : B ss, exists ls, exists ls',
+        nth_error sfuncs n = Some ss 
+        /\ FM.find n impures = Some ls 
+        /\ fold_args_update se ls = Some ls'
+        /\ i' = FM.add n ls' impures.
+  Proof.
+    clear. induction k; simpl.
+    congruence.
+    intros h v. specialize (IHk (hlist_tl h) v).
+    rewrite (hlist_eta _ h) in *.
+    generalize dependent (hlist_hd h). simpl.
+    case_eq (FM.find a impures); intros; eauto 10.
+
+    assert (exists k, nth_error sfuncs a = Some k).
+    generalize y. clear.
+    destruct (nth_error sfuncs a); [ eauto | destruct 1 ]. 
+    destruct H1.
+    generalize dependent y.
+    rewrite H1. intro.
+    case_eq (fold_args_update y l); intros; eauto 10.
+    inversion H2; subst.
+    eauto 10.
+  Qed.
+
+End search_read_write.
+
 Module Evaluator (B : Heap) (ST : SepTheoryX.SepTheoryXType B).
   Module Import SEP := SepExpr B ST.
 
@@ -23,237 +261,342 @@ Module Evaluator (B : Heap) (ST : SepTheoryX.SepTheoryXType B).
                            | _ => None
                          end
        |}.
+
+    (** * Bytes *)
+    Section ByteAccess.
+      Variable byteIndex : nat.
+      Definition byteType : type :=
+        {| Impl := B
+          ; Eq := fun x y => match weq x y with
+                               | left pf => Some pf
+                               | _ => None
+                             end
+        |}.
+
+      Hypothesis byte_ptr : byteIndex <> ptrIndex.
+
+      Definition btypes := 
+        updatePosition ptrIndex ptrType (updatePosition byteIndex byteType types').
+
+      Lemma ptrType_get : tvarD btypes (tvType ptrIndex) = B.addr.
+        unfold btypes, tvarD. rewrite updatePosition_eq. reflexivity.
+      Qed.
+
+      Definition exprD_ptr (funcs : functions btypes) (uvars vars : env btypes)
+        (e : expr btypes) : option B.addr :=
+        match ptrType_get in _ = t return option t with
+          | refl_equal => exprD funcs uvars vars e (tvType ptrIndex)
+        end.
+
+      Lemma byteType_get : tvarD btypes (tvType byteIndex) = B.
+        unfold btypes, tvarD. rewrite updatePosition_neq; auto;
+        rewrite updatePosition_eq; auto. congruence.
+      Qed.
+
+      Definition exprD_byte (funcs : functions btypes) (uvars vars : env btypes)
+        (e : expr btypes) : option B :=
+        match byteType_get in _ = t return option t with
+          | refl_equal => exprD funcs uvars vars e (tvType byteIndex)
+        end.
+
+
+
+      Record SymEval_byte (Predicate : ssignature btypes (tvType pcIndex) (tvType stateIndex))
+        : Type :=
+        { sym_read_byte  : 
+          forall (hyps args : list (expr btypes)) (p : expr btypes), option (expr btypes)
+            ; sym_write_byte : 
+            forall (hyps args : list (expr btypes)) (p v : expr btypes),
+              option (list (expr btypes))
+              ; sym_read_byte_correct : forall funcs args uvars vars cs hyps pe ve m stn P,
+                sym_read_byte hyps args pe = Some ve ->
+                AllProvable funcs uvars vars hyps ->
+                match 
+                  applyD (@exprD _ funcs uvars vars) (SDomain Predicate) args _ (SDenotation Predicate)
+                  with
+                  | None => False
+                  | Some p => ST.satisfies cs (ST.star p P) stn m
+                end ->
+                match exprD_ptr funcs uvars vars pe , exprD_byte funcs uvars vars ve with
+                  | Some p , Some v =>
+                    ST.HT.smem_get p m = Some v
+                  | _ , _ => False
+                end
+                ; sym_write_byte_correct : forall funcs args uvars vars P cs hyps pe ve v m stn args',
+                  sym_write_byte hyps args pe ve = Some args' ->
+                  AllProvable funcs uvars vars hyps ->
+                  exprD_byte funcs uvars vars ve = Some v ->
+                  match
+                    applyD (@exprD _ funcs uvars vars) (SDomain Predicate) args _ (SDenotation Predicate)
+                    with
+                    | None => False
+                    | Some p => ST.satisfies cs (ST.star p P) stn m
+                  end ->
+                  match exprD_ptr funcs uvars vars pe with
+                    | Some p =>
+                      match 
+                        applyD (@exprD _ funcs uvars vars) (SDomain Predicate) args' _ (SDenotation Predicate)
+                        with
+                        | None => False
+                        | Some pr => 
+                          ST.satisfies cs (ST.star pr P) stn (ST.HT.smem_set p v m)
+                      end
+                    | _ => False
+                  end
+        }.
+
+      Definition defaultSymEval_byte (P : ssignature btypes (tvType pcIndex) (tvType stateIndex))
+        : SymEval_byte P.
+      refine (
+        {| sym_read_byte          := fun _ _ _ => None
+          ; sym_write_byte         := fun _ _ _ _ => None
+            ; sym_read_byte_correct  := _
+            ; sym_write_byte_correct := _
+        |}); 
+      abstract (simpl; intros; congruence).
+      Defined.
+    End ByteAccess.
+
+    (** * Words *)
+    Section WordAccess.
+      Variable wordIndex : nat.
+      Definition wordType : type :=
+        {| Impl := W
+          ; Eq := fun x y => match weq x y with
+                               | left pf => Some pf
+                               | _ => None
+                             end
+        |}.
+
+      Hypothesis word_ptr : wordIndex <> ptrIndex.
+
+      Definition wtypes := 
+        updatePosition ptrIndex ptrType (updatePosition wordIndex wordType types').
+
+      Lemma ptrType_get_w : tvarD wtypes (tvType ptrIndex) = B.addr.
+        unfold wtypes, tvarD. rewrite updatePosition_eq. reflexivity.
+      Qed.
+
+      Definition exprD_ptr_w (funcs : functions wtypes) (uvars vars : env wtypes)
+        (e : expr wtypes) : option B.addr :=
+        match ptrType_get_w in _ = t return option t with
+          | refl_equal => exprD funcs uvars vars e (tvType ptrIndex)
+        end.
+
+      Lemma wordType_get_w : tvarD wtypes (tvType wordIndex) = W.
+        unfold wtypes, tvarD. rewrite updatePosition_neq; auto;
+        rewrite updatePosition_eq; auto. congruence.
+      Qed.
+
+      Definition exprD_word (funcs : functions wtypes) (uvars vars : env wtypes)
+        (e : expr wtypes) : option W :=
+        match wordType_get_w in _ = t return option t with
+          | refl_equal => exprD funcs uvars vars e (tvType wordIndex)
+        end.
+
+      Record SymEval_word (Predicate : ssignature wtypes (tvType pcIndex) (tvType stateIndex))
+        : Type :=
+        { sym_read_word  : 
+          forall (hyps args : list (expr wtypes)) (p : expr wtypes), option (expr wtypes)
+        ; sym_write_word : 
+          forall (hyps args : list (expr wtypes)) (p v : expr wtypes),
+            option (list (expr wtypes))
+         ; sym_read_word_correct : forall funcs args uvars vars cs hyps pe ve m stn P,
+           sym_read_word hyps args pe = Some ve ->
+           AllProvable funcs uvars vars hyps ->
+           match 
+             applyD (exprD funcs uvars vars) (SDomain Predicate) args _ (SDenotation Predicate)
+             with
+             | None => False
+             | Some p => ST.satisfies cs (ST.star p P) stn m
+           end ->
+           match exprD_ptr_w funcs uvars vars pe , exprD_word funcs uvars vars ve with
+             | Some p , Some v =>
+               ST.HT.smem_get_word (IL.implode stn) p m = Some v
+             | _ , _ => False
+           end
+         ; sym_write_word_correct : forall funcs args uvars vars P cs hyps pe ve v m stn args',
+           sym_write_word hyps args pe ve = Some args' ->
+           AllProvable funcs uvars vars hyps ->
+           exprD_word funcs uvars vars ve = Some v ->
+           match
+             applyD (@exprD _ funcs uvars vars) (SDomain Predicate) args _ (SDenotation Predicate)
+             with
+             | None => False
+             | Some p => ST.satisfies cs (ST.star p P) stn m
+           end ->
+           match exprD_ptr_w funcs uvars vars pe with
+             | Some p =>
+               match 
+                 applyD (@exprD _ funcs uvars vars) (SDomain Predicate) args' _ (SDenotation Predicate)
+                 with
+                 | None => False
+                 | Some pr => 
+                   ST.satisfies cs (ST.star pr P) stn (ST.HT.smem_set_word (IL.explode stn) p v m)
+               end
+             | _ => False
+           end
+      }.
+
+      Definition defaultSymEval_word (P : ssignature wtypes (tvType pcIndex) (tvType stateIndex))
+        : SymEval_word P.
+      refine (
+        {| sym_read_word          := fun _ _ _ => None
+         ; sym_write_word         := fun _ _ _ _ => None
+         ; sym_read_word_correct  := _
+         ; sym_write_word_correct := _
+        |}); 
+      abstract (simpl; intros; congruence).
+      Defined.
+
+      (** * The full tactic *)
+      Variable sfuncs : list (ssignature wtypes (tvType pcIndex) (tvType stateIndex)).
+
+      Variable known : list nat. 
+      Variable evals : hlist (fun n : nat => match nth_error sfuncs n with
+                                               | None => Empty_set 
+                                               | Some ss => SymEval_word ss
+                                             end) known.
+
+      Definition symeval_read_word (hyps : list (expr wtypes)) (p : expr wtypes) 
+        (s : SHeap wtypes (tvType pcIndex) (tvType stateIndex))
+        : option (expr wtypes) :=
+        let hyps := hyps ++ pures s in
+        let reader ss (seb : SymEval_word ss) args := 
+          sym_read_word seb hyps args p
+        in
+        fold_known _ _ reader (impures s) evals.
+
+      Theorem symeval_read_word_correct : forall cs stn hyps funcs pe ve s uvars vars m,
+        symeval_read_word hyps pe s = Some ve ->
+        AllProvable funcs uvars vars hyps ->
+        (exists sm, 
+             ST.satisfies cs (sexprD funcs sfuncs uvars vars (sheapD s)) stn sm
+          /\ ST.HT.satisfies sm m) ->
+        match exprD_ptr_w funcs uvars vars pe , exprD_word funcs uvars vars ve with
+          | Some p , Some v => 
+            ST.HT.mem_get_word (IL.implode stn) p m = Some v
+          | _ , _ => False
+        end.
+      Proof.
+        unfold symeval_read_word. intros.
+        eapply fold_known_correct in H.
+        do 5 destruct H. destruct H1.
+        intuition.
+
+        generalize (sheapD_pures _ _ _ _ _ H); intros.
+
+        eapply sheapD_pull_impure 
+          with (funcs := funcs) (sfuncs := sfuncs) (a := uvars) (c := vars0) (cs := cs)
+            in H1.
+        eapply starred_In in H3.
+        destruct H3. rewrite H3 in H1.
+
+        eapply sym_read_word_correct 
+          with (funcs := funcs) (uvars := uvars) (vars := vars0) (cs := cs) (stn := stn) (m := x4)
+            in H6.
+        3: instantiate (1 := sexprD funcs sfuncs uvars vars0 (Star
+          (sheapD
+            {|
+              impures := FM.remove x (impures s);
+              pures := pures s;
+              other := other s |})
+          (starred (Func x) x5 Emp))).
+        destruct (exprD_ptr_w funcs uvars vars0 pe); auto.
+        destruct (exprD_word funcs uvars vars0 ve); auto.
+        erewrite ST.HT.satisfies_get_word; eauto.
+
+        eapply AllProvable_app; auto.
+
+        unfold heq in *.
+        rewrite H1 in H. simpl in *. rewrite ST.heq_star_comm in H.
+        rewrite H2 in *. rewrite ST.heq_star_assoc in H.
+        rewrite ST.heq_star_comm in H. rewrite ST.heq_star_assoc in H.
+        generalize H. clear.
+        match goal with 
+          | [ |- context [ applyD ?A ?B ?C ?D ?E ] ] =>
+            destruct (applyD A B C D E)
+        end; auto.
+        clear. intros.
+        eapply ST.satisfies_star in H. do 2 destruct H. intuition.
+        eapply ST.satisfies_pure in H0. PropXTac.propxFo.
+      Qed.
+
+      Definition symeval_write_word (hyps : list (expr wtypes)) (p v : expr wtypes) 
+        (s : SHeap wtypes (tvType pcIndex) (tvType stateIndex))
+        : option (SHeap wtypes (tvType pcIndex) (tvType stateIndex)) :=
+        let hyps := hyps ++ pures s in
+        let writer _ seb args := 
+          sym_write_word seb hyps args p v
+        in
+        match fold_known_update _ _ writer (impures s) evals with
+          | None => None
+          | Some i' => Some {| impures := i' ; pures := pures s ; other := other s |}
+        end.
+
+      Theorem symeval_write_word_correct : forall cs stn hyps funcs pe ve s s' uvars vars m,
+        symeval_write_word hyps pe ve s = Some s' ->
+        AllProvable funcs uvars vars hyps ->
+        (exists sm, 
+             ST.satisfies cs (sexprD funcs sfuncs uvars vars (sheapD s)) stn sm
+          /\ ST.HT.satisfies sm m) ->
+        match exprD_ptr_w funcs uvars vars pe , exprD_word funcs uvars vars ve with
+          | Some p , Some v =>
+            exists sm, 
+                 ST.satisfies cs (sexprD funcs sfuncs uvars vars (sheapD s')) stn sm
+              /\ ST.HT.satisfies sm (ST.HT.mem_set_word (IL.explode stn) p v m)
+          | _ , _ => False
+        end.
+      Proof.
+        unfold symeval_write_word. intros.
+        generalize dependent H.
+        match goal with
+          | [ |- context [ fold_known_update ?A ?B ?C ?D ?E ] ] =>
+            case_eq (fold_known_update A B C D E); intros; try congruence
+        end.
+        eapply fold_known_update_correct in H.
+        do 5 destruct H. destruct H1.
+        intuition. inversion H2; clear H2; subst. 
+        
+        eapply fold_args_update_correct in H5.
+        repeat match goal with
+                 | [ H : exists x, _ |- _ ] => destruct H
+               end. intuition; subst.
+        generalize (sheapD_pures _ _ _ _ _ H3).
+        rewrite sheapD_pull_impure in H3 by eauto.
+        assert (In x7 (x5 ++ x7 :: x6)). 
+        apply in_or_app; right; simpl; auto.
+        eapply starred_In in H5.
+        destruct H5. rewrite H5 in H3.
+        rewrite <- heq_star_assoc in H3. rewrite heq_star_comm in H3.
+        
+        simpl in *. rewrite H1 in *.
+        intros.
+        eapply sym_write_word_correct in H2; eauto.
+        2: apply AllProvable_app; eauto.
+
+        Focus 2.
+
+        generalize dependent H3.
+        match goal with
+          | [ |- context [ applyD ?A ?B ?C ?D ?E ] ] =>
+            case_eq (applyD A B C D E)
+        end. intros.
+        generalize (sym_write_word_correct).
+        
+
+      Admitted.
+
+    End WordAccess.
+
 (*
-    Variable wordIndex : nat.
-    Definition wordType : type :=
-      {| Impl := W
-       ; Eq := fun x y => match weq x y with
-                           | left pf => Some pf
-                           | _ => None
-                         end
-       |}.
-*)
-    Variable byteIndex : nat.
-    Definition byteType : type :=
-      {| Impl := B
-       ; Eq := fun x y => match weq x y with
-                            | left pf => Some pf
-                            | _ => None
-                          end
-       |}.
-
-    Fixpoint updatePosition {T} (n : nat) (v : T) (ls : list T) : list T :=
-      match n , ls with
-        | 0 , nil => v :: nil
-        | 0 , _ :: b => v :: b 
-        | S n , nil => v :: updatePosition n v nil
-        | S n , a :: b => a :: updatePosition n v b
-      end.
-
-    Lemma updatePosition_tvarD_eq : forall n types' t,
-      tvarD (updatePosition n t types') (tvType n) = Impl t.
-    Proof.
-      clear. unfold tvarD.
-      induction n; simpl; destruct types'; eauto.
-    Defined.
-
-(*
-    Lemma updatePosition_tvarD_neq : forall t n types' m,
-      n <> m ->
-      tvarD (updatePosition m t types') (tvType n) = tvarD types' (tvType n).
-    Proof.
-      clear.
-      induction n; destruct types'; destruct m; simpl; intros; try solve [ exfalso; omega ]; auto.
-      unfold tvarD in *. rewrite IHn; eauto. omega.      
-    Defined.
-*)
-
-
-    Definition types := 
-(*      updatePosition stateIndex stateType (updatePosition pcIndex pcType (
-        *)
-      updatePosition ptrIndex ptrType (updatePosition byteIndex byteType types').
-
-    Lemma ptrType_get : tvarD types (tvType ptrIndex) = B.addr.
-      unfold types. apply updatePosition_tvarD_eq.
-    Qed.
-
-
-    Definition exprD_ptr (funcs : functions types) (uvars vars : env types) (e : expr types) : 
-      option B.addr :=
-      match ptrType_get in _ = t return option t with
-        | refl_equal => 
-          @exprD types funcs uvars vars e (tvType ptrIndex)
-      end.
-
-    Lemma byteType_get : tvarD types (tvType byteIndex) = B.
-      unfold types. 
-    Admitted.
-
-
-    Definition exprD_byte (funcs : functions types) (uvars vars : env types) (e : expr types) : 
-      option B :=
-      match byteType_get in _ = t return option t with
-        | refl_equal =>
-          @exprD types funcs uvars vars e (tvType byteIndex)
-      end.
-
-    Record SymEval_byte (Predicate : ssignature types (tvType pcIndex) (tvType stateIndex))
-      : Type :=
-    { sym_read_byte  : 
-      forall (hyps args : list (expr types)) (p : expr types), option (expr types)
-    ; sym_write_byte : 
-      forall (hyps args : list (expr types)) (p v : expr types),
-        option (list (expr types))
-    ; sym_read_byte_correct : forall funcs args uvars vars cs hyps pe ve m stn P,
-      sym_read_byte hyps args pe = Some ve ->
-      AllProvable funcs uvars vars hyps ->
-      match 
-        applyD (@exprD _ funcs uvars vars) (SDomain Predicate) args _ (SDenotation Predicate)
-        with
-        | None => False
-        | Some p => ST.satisfies cs (ST.star p P) stn m
-      end ->
-      match exprD_ptr funcs uvars vars pe , exprD_byte funcs uvars vars ve with
-        | Some p , Some v =>
-          ST.HT.smem_get p m = Some v
-        | _ , _ => False
-      end
-    ; sym_write_byte_correct : forall funcs args uvars vars P cs hyps pe ve v m stn args',
-      sym_write_byte hyps args pe ve = Some args' ->
-      AllProvable funcs uvars vars hyps ->
-      exprD_byte funcs uvars vars ve = Some v ->
-      match
-        applyD (@exprD _ funcs uvars vars) (SDomain Predicate) args _ (SDenotation Predicate)
-        with
-        | None => False
-        | Some p => ST.satisfies cs (ST.star p P) stn m
-      end ->
-      match exprD_ptr funcs uvars vars pe with
-        | Some p =>
-          match 
-            applyD (@exprD _ funcs uvars vars) (SDomain Predicate) args' _ (SDenotation Predicate)
-            with
-            | None => False
-            | Some pr => 
-              ST.satisfies cs (ST.star pr P) stn (ST.HT.smem_set p v m)
-          end
-        | _ => False
-      end
-    }.
-
-    Definition defaultSymEval_byte (P : ssignature types (tvType pcIndex) (tvType stateIndex))
-      : SymEval_byte P.
-    refine (
-      {| sym_read_byte          := fun _ _ _ => None
-       ; sym_write_byte         := fun _ _ _ _ => None
-       ; sym_read_byte_correct  := _
-       ; sym_write_byte_correct := _
-       |}); 
-    abstract (simpl; intros; congruence).
-    Defined.
 
     (** The full tactic **)
+    (** TODO : I really want to abstract this so that I don't have to rewrite it for
+     ** each read and write size
+     **)
+
     Variable sfuncs : list (ssignature types (tvType pcIndex) (tvType stateIndex)).
-
-    Section search_read.
-      Variable T : Type.
-      Variable F : forall s, SymEval_byte s -> list (expr types) -> option T.
-
-      Section arg.
-        Variable ss : ssignature types (tvType pcIndex) (tvType stateIndex).
-        Variable se : SymEval_byte ss.
-        
-        Fixpoint fold_args (es : list (list (expr types))) : option T :=
-          match es with 
-            | nil => None
-            | a :: b => 
-              match F se a with
-                | None => fold_args b
-                | Some r => Some r
-              end
-          end.
-        
-        Theorem fold_args_correct : forall es v,
-          fold_args es = Some v ->
-          exists k, In k es /\ F se k = Some v.
-        Proof.
-          clear. induction es.
-          simpl; congruence.
-          simpl. case_eq (F se a); intros.
-          inversion H0. subst. eauto.
-          eapply IHes in H0. destruct H0.
-          exists x. tauto.
-        Qed.          
-      End arg.
-
-      Variable impures : FM.t (list (list (expr types))).
-
-      Fixpoint fold_known (k : list nat) :
-        hlist (fun n : nat => match nth_error sfuncs n with
-                                | None => Empty_set 
-                                | Some ss => SymEval_byte ss
-                              end) k
-        -> option T :=
-        match k as k 
-          return hlist (fun n : nat => match nth_error sfuncs n with
-                                         | None => Empty_set 
-                                         | Some ss => SymEval_byte ss
-                                       end) k
-                 -> option T
-          with
-          | nil => fun _ => None
-          | a :: b => fun ss =>
-            match FM.find a impures with
-              | None => fold_known (hlist_tl ss)
-              | Some argss =>
-                match nth_error sfuncs a as ss
-                  return match ss with
-                           | None => Empty_set 
-                           | Some ss => SymEval_byte ss
-                         end -> option T
-                  with
-                  | Some _ => fun se =>
-                    match fold_args se argss with
-                      | None => fold_known (hlist_tl ss)
-                      | Some r => Some r
-                    end
-                  | None => fun err => match err with end
-                end (hlist_hd ss)
-            end
-        end.
-      
-      Theorem fold_known_correct : forall k
-        (h : hlist (fun n : nat => match nth_error sfuncs n with
-                                     | None => Empty_set 
-                                     | Some ss => SymEval_byte ss
-                                   end) k) v,
-        @fold_known k h = Some v ->
-        exists n, exists ss,
-          exists se :  SymEval_byte ss, exists ls, exists args, 
-               nth_error sfuncs n = Some ss 
-            /\ FM.find n impures = Some ls 
-            /\ In args ls 
-            /\ F se args = Some v.
-      Proof.
-        induction k; simpl.
-          congruence.
-          intros h v. specialize (IHk (hlist_tl h) v).
-          rewrite (hlist_eta _ h) in *.
-          generalize dependent (hlist_hd h). simpl.
-          case_eq (FM.find a impures); intros; eauto 10.
-
-          assert (exists k, nth_error sfuncs a = Some k).
-          generalize y. clear.
-          destruct (nth_error sfuncs a); [ eauto | destruct 1 ]. 
-          destruct H1.
-          generalize dependent y.
-          rewrite H1. intro.
-          case_eq (fold_args y l); intros; eauto 10.
-          inversion H2; subst.
-          eapply fold_args_correct in H0. destruct H0; eauto 10.
-      Qed.
-    End search_read.
 
     Variable known : list nat. 
     Variable evals : hlist (fun n : nat => match nth_error sfuncs n with
@@ -325,118 +668,6 @@ Module Evaluator (B : Heap) (ST : SepTheoryX.SepTheoryXType B).
       eapply ST.satisfies_pure in H0. PropXTac.propxFo.
     Qed.
 
-    Section search_write.
-      Variable T : Type.
-      Variable F : forall s, SymEval_byte s -> T -> option T.
-
-      Section arg.
-        Variable ss : ssignature types (tvType pcIndex) (tvType stateIndex).
-        Variable se : SymEval_byte ss.
-        
-        Fixpoint fold_args_update (es : list T) : option (list T) :=
-          match es with 
-            | nil => None
-            | a :: b => 
-              match F se a with
-                | None => match fold_args_update b with
-                            | None => None
-                            | Some b => Some (a :: b)
-                          end
-                | Some r => Some (r :: b)
-              end
-          end.
-        
-        Theorem fold_args_update_correct : forall es es',
-          fold_args_update es = Some es' ->
-          exists pre, exists post, exists k, exists k',
-            es = pre ++ k :: post /\
-            F se k = Some k' /\
-            es' = pre ++ k' :: post.
-        Proof.
-          clear. induction es.
-          simpl; congruence.
-          simpl. case_eq (F se a); intros.
-          inversion H0. subst. do 4 eexists; intuition eauto.
-          instantiate (2 := nil). reflexivity. reflexivity.
-
-          generalize dependent H0.
-          case_eq (fold_args_update es); intros.
-          inversion H1; subst. eapply IHes in H0.
-          do 4 destruct H0. exists (a :: x). exists x0.
-          eexists; eexists; intuition; subst; eauto. reflexivity.
-
-          congruence.
-        Qed.          
-      End arg.
-
-      Variable impures : FM.t (list T).
-
-      Fixpoint fold_known_update (k : list nat) :
-        hlist (fun n : nat => match nth_error sfuncs n with
-                                | None => Empty_set 
-                                | Some ss => SymEval_byte ss
-                              end) k
-        -> option (FM.t (list T)) :=
-        match k as k 
-          return hlist (fun n : nat => match nth_error sfuncs n with
-                                         | None => Empty_set 
-                                         | Some ss => SymEval_byte ss
-                                       end) k
-                 -> option (FM.t (list T))
-          with
-          | nil => fun _ => None
-          | a :: b => fun ss =>
-            match FM.find a impures with
-              | None => fold_known_update (hlist_tl ss)
-              | Some argss =>
-                match nth_error sfuncs a as ss
-                  return match ss with
-                           | None => Empty_set 
-                           | Some ss => SymEval_byte ss
-                         end -> option (FM.t (list T))
-                  with
-                  | Some _ => fun se =>
-                    match fold_args_update se argss with
-                      | None => fold_known_update (hlist_tl ss)
-                      | Some r => Some (FM.add a r impures) (* this is a replace *)
-                    end
-                  | None => fun err => match err with end
-                end (hlist_hd ss)
-            end
-        end.
-      
-      Theorem fold_known_update_correct : forall k
-        (h : hlist (fun n : nat => match nth_error sfuncs n with
-                                     | None => Empty_set 
-                                     | Some ss => SymEval_byte ss
-                                   end) k) i',
-        @fold_known_update k h = Some i' ->
-        exists n, exists ss,
-          exists se : SymEval_byte ss, exists ls, exists ls',
-               nth_error sfuncs n = Some ss 
-            /\ FM.find n impures = Some ls 
-            /\ fold_args_update se ls = Some ls'
-            /\ i' = FM.add n ls' impures.
-      Proof.
-        induction k; simpl.
-          congruence.
-          intros h v. specialize (IHk (hlist_tl h) v).
-          rewrite (hlist_eta _ h) in *.
-          generalize dependent (hlist_hd h). simpl.
-          case_eq (FM.find a impures); intros; eauto 10.
-
-          assert (exists k, nth_error sfuncs a = Some k).
-          generalize y. clear.
-          destruct (nth_error sfuncs a); [ eauto | destruct 1 ]. 
-          destruct H1.
-          generalize dependent y.
-          rewrite H1. intro.
-          case_eq (fold_args_update y l); intros; eauto 10.
-          inversion H2; subst.
-          eauto 10.
-      Qed.
-    End search_write.
-
     Definition symeval_write_byte (hyps : list (expr types)) (p v : expr types) 
       (s : SHeap types (tvType pcIndex) (tvType stateIndex))
       : option (SHeap types (tvType pcIndex) (tvType stateIndex)) :=
@@ -464,7 +695,7 @@ Module Evaluator (B : Heap) (ST : SepTheoryX.SepTheoryXType B).
       end.
     Proof.
     Admitted.
-
+*)
   End typed.
 End Evaluator.
 
