src/Bedrock.v
@@ -1,9 +1,9 @@
 Require Export String List NArith.
 
-Require Export Nomega Word IL LabelMap PropX PropXTac XCAP Structured StructuredModule Linker Programming.
-
 Require Export Heaps SepTheoryX SepIL.
 
-Require Export SepTac.
+Require Export Nomega Word IL LabelMap PropX PropXTac XCAP Structured StructuredModule Linker Programming.
+
+Require Export Bedrock.SepTac.
 
 Open Scope string_scope.
